fullstackbetree refinement skeleton

Splinter/AllocationsLayer/AllocationBetreeRefinement.i.dfy
@@ -2,10 +2,13 @@
 // SPDX-License-Identifier: BSD-2-Clause
 
 include "AllocationBetree.i.dfy"
+include "../Betree/LikesBetreeRefinement.i.dfy"
 
 // a conditional refinement where it only refines if newly allocated AUs are fresh
 module AllocationBetreeRefinement {
+  import opened StampedMod
   import opened AllocationBetreeMod
+  import LikesBetreeRefinement
   import LikesBetreeMod
 
   function I(v: Variables) : LikesBetreeMod.Variables
@@ -13,10 +16,15 @@ module AllocationBetreeRefinement {
     v.likesVars
   }
 
+  function IStampedBetree(image: StampedBetree) : LikesBetreeMod.StampedBetree
+  {
+    Stamped(image.value.branched, image.seqEnd)
+  }
+
   predicate Inv(v: Variables)
   {
     // placeholder
-    && true
+    && LikesBetreeRefinement.Inv(v.likesVars)
   }
 
   predicate IsFresh(v: Variables, aus: set<AU>)
@@ -27,21 +35,40 @@ module AllocationBetreeRefinement {
     && G.ToAUs(v.allocBranchDiskView.Representation()) !! aus 
   }
 
-  lemma InvNext(v: Variables, v': Variables, lbl: TransitionLabel)
-    requires Inv(v)
-    requires Next(v, v', lbl)
-    ensures Inv(v')
+  predicate FreshLabel(v: Variables,lbl: TransitionLabel)
   {
+   && lbl.InternalAllocationsLabel? ==> IsFresh(v, lbl.allocs)
   }
+
+  predicate ValidStampedBetree(stamped: StampedBetree)
+  {
+    && LikesBetreeRefinement.ValidStampedBetree(IStampedBetree(stamped))
+  }
+
+  lemma InitRefines(v: Variables, stamped: StampedBetree)
+    requires Init(v, stamped)
+    requires ValidStampedBetree(stamped)
+    ensures Inv(v)
+    ensures LikesBetreeMod.Init(I(v), IStampedBetree(stamped))
+  {
+    LikesBetreeRefinement.InitRefines(v.likesVars, IStampedBetree(stamped));
+  }
+
+  // lemma InvNext(v: Variables, v': Variables, lbl: TransitionLabel)
+  //   requires Inv(v)
+  //   requires Next(v, v', lbl)
+  //   ensures Inv(v')
+  // {
+  // }
 
   lemma NextRefines(v: Variables, v': Variables, lbl: TransitionLabel)
     requires Inv(v)
     requires Next(v, v', lbl)
-    requires lbl.InternalAllocationsLabel? ==> IsFresh(v, lbl.allocs)
+    requires FreshLabel(v, lbl)
     ensures Inv(v')
     ensures LikesBetreeMod.Next(I(v), I(v'), lbl.I())
   {
-    InvNext(v, v', lbl);
+    // InvNext(v, v', lbl);
     assume false;
   }
 }
