Splinter/Betree/LikesBetreeRefinement.i.dfy
@@ -2,10 +2,12 @@
 // SPDX-License-Identifier: BSD-2-Clause
 
 include "LikesBetree.i.dfy"
+include "BranchedBetreeRefinement.i.dfy"
 
 // a conditional refinement where it only refines if newly allocated AUs are fresh
 module LikesBetreeRefinement {
   import opened LikesBetreeMod
+  import BranchedBetreeRefinement
   import BranchedBetreeMod
 
   function I(v: Variables) : BranchedBetreeMod.Variables
@@ -16,15 +18,29 @@ module LikesBetreeRefinement {
   predicate Inv(v: Variables)
   {
     // placeholder
-    && true
+    && BranchedBetreeRefinement.Inv(v.branchedVars)
   }
 
-  lemma InvNext(v: Variables, v': Variables, lbl: TransitionLabel)
-    requires Inv(v)
-    requires Next(v, v', lbl)
-    ensures Inv(v')
+  predicate ValidStampedBetree(stamped: StampedBetree)
   {
+    && BranchedBetreeRefinement.InvBranchedBetree(stamped.value)
   }
+
+  lemma InitRefines(v: Variables, stamped: StampedBetree)
+    requires Init(v, stamped)
+    requires ValidStampedBetree(stamped)
+    ensures Inv(v)
+    ensures BranchedBetreeMod.Init(I(v), stamped)
+  {
+    BranchedBetreeRefinement.InitRefines(v.branchedVars, stamped);
+  }
+
+  // lemma InvNext(v: Variables, v': Variables, lbl: TransitionLabel)
+  //   requires Inv(v)
+  //   requires Next(v, v', lbl)
+  //   ensures Inv(v')
+  // {
+  // }
 
   lemma NextRefines(v: Variables, v': Variables, lbl: TransitionLabel)
     requires Inv(v)
@@ -32,7 +48,7 @@ module LikesBetreeRefinement {
     ensures Inv(v')
     ensures BranchedBetreeMod.Next(I(v), I(v'), lbl.I())
   {
-    InvNext(v, v', lbl);
+    // InvNext(v, v', lbl);
     assume false;
   }
 }
