Splinter/AllocationsLayer/FullStackBetreeRefinement.i.dfy
@@ -1,0 +1,150 @@
+// Copyright 2018-2021 VMware, Inc., Microsoft Inc., Carnegie Mellon University, ETH Zurich, and University of Washington
+// SPDX-License-Identifier: BSD-2-Clause
+
+include "../CoordinationLayer/CrashTolerantMap.i.dfy"
+include "CoordinationBetree.i.dfy"
+include "AllocationBetreeRefinement.i.dfy"
+include "../Betree/LikesBetreeRefinement.i.dfy"
+include "../Betree/BranchedBetreeRefinement.i.dfy"
+include "../Betree/LinkedBetreeRefinement.i.dfy"
+include "../Betree/FilteredBetreeRefinement.i.dfy"
+include "../Betree/PivotBetreeRefinement.i.dfy"
+include "../Betree/PagedBetreeRefinement.i.dfy"
+
+module FullStackBetreeRefinement {
+  import opened Options
+  import opened StampedMod
+  import CoordinationBetree
+  import AllocationBetreeMod
+  import AllocationBetreeRefinement
+  import LikesBetreeRefinement
+  import BranchedBetreeRefinement
+  import LinkedBetreeRefinement
+  import FilteredBetreeRefinement
+  import PivotBetreeRefinement
+  import PagedBetreeRefinement
+  import AbstractMap
+  import CrashTolerantMap
+
+  function ILbl(lbl: CoordinationBetree.TransitionLabel) : CrashTolerantMap.TransitionLabel
+  {
+    match lbl
+      case LoadEphemeralFromPersistentLabel(endLsn) => CrashTolerantMap.LoadEphemeralFromPersistentLabel(endLsn)
+      case PutRecordsLabel(records) => CrashTolerantMap.PutRecordsLabel(records)
+      case QueryLabel(endLsn, key, value) => CrashTolerantMap.QueryLabel(endLsn, key, value)
+      case FreezeAsLabel(_) => CrashTolerantMap.InternalLabel()
+      case InternalLabel(_, _) => CrashTolerantMap.InternalLabel()
+      case CommitStartLabel(newBoundaryLsn) => CrashTolerantMap.CommitStartLabel(newBoundaryLsn) 
+      case CommitCompleteLabel() => CrashTolerantMap.CommitCompleteLabel()
+      case CrashLabel() => CrashTolerantMap.CrashLabel()
+  }
+
+  function AllocLbl(v: CoordinationBetree.Variables, v': CoordinationBetree.Variables, lbl: CoordinationBetree.TransitionLabel) : AllocationBetreeMod.TransitionLabel
+    requires CoordinationBetree.Next(v, v', lbl)
+  {
+    match lbl
+      case PutRecordsLabel(records) => AllocationBetreeMod.PutLabel(records)
+      case QueryLabel(endLsn, key, value) => AllocationBetreeMod.QueryLabel(endLsn, key, value)
+      case FreezeAsLabel(unobserved) => AllocationBetreeMod.FreezeAsLabel(v'.inFlight.value, lbl.unobserved)
+      case InternalLabel(allocs, deallocs) => AllocationBetreeMod.InternalAllocationsLabel(allocs, deallocs)
+      case _ => AllocationBetreeMod.InternalAllocationsLabel({}, {}) // no op label
+  }
+
+  predicate Inv(v: CoordinationBetree.Variables)
+  {
+    && (v.ephemeral.Known? ==> AllocationBetreeRefinement.Inv(v.ephemeral.v))
+    && (v.inFlight.Some? ==> v.inFlight.value.value.branched.Acyclic())
+    && v.persistent.value.branched.Acyclic()
+  }
+
+  function IBetree(betree: AllocationBetreeMod.Variables) : AbstractMap.Variables
+    requires AllocationBetreeRefinement.Inv(betree)
+  {
+    var likesBetree := AllocationBetreeRefinement.I(betree);
+    var branchedBetree := LikesBetreeRefinement.I(likesBetree);
+    var linkedBetree := BranchedBetreeRefinement.I(branchedBetree);
+    var filteredBetree := LinkedBetreeRefinement.I(linkedBetree);
+    var pivotBetree := FilteredBetreeRefinement.I(filteredBetree);
+    var pagedBetree := PivotBetreeRefinement.I(pivotBetree);
+    var abstractMap := PagedBetreeRefinement.I(pagedBetree);
+    abstractMap
+  }
+
+  function IBetreeImage(image: AllocationBetreeMod.StampedBetree) : CrashTolerantMap.StoreImage
+    requires image.value.branched.Acyclic()
+  {
+    var branchedImage := AllocationBetreeRefinement.IStampedBetree(image);
+    var linkedImage := BranchedBetreeRefinement.IStampedBetree(branchedImage);
+    var filteredImage := LinkedBetreeRefinement.IStampedBetree(linkedImage);
+    var pivotImage := FilteredBetreeRefinement.IStampedBetree(filteredImage);
+    var pagedImage := PivotBetreeRefinement.IStampedBetree(pivotImage);
+    var mapImage := PagedBetreeRefinement.IStampedBetree(pagedImage);
+    mapImage
+  }
+
+  function IEphemeral(ephemeral: CoordinationBetree.Ephemeral) : CrashTolerantMap.Ephemeral
+    requires ephemeral.Known? ==> AllocationBetreeRefinement.Inv(ephemeral.v)
+  {
+    if ephemeral.Unknown? then CrashTolerantMap.Unknown
+    else CrashTolerantMap.Known(IBetree(ephemeral.v))
+  }
+
+  function I(v: CoordinationBetree.Variables) : CrashTolerantMap.Variables
+    requires Inv(v)
+  {
+    CrashTolerantMap.Variables(
+      IBetreeImage(v.persistent), 
+      IEphemeral(v.ephemeral),
+      if v.inFlight.Some? then Some(IBetreeImage(v.inFlight.value)) else None
+    )
+  }
+
+  // lemma InvNext(v: CoordinationBetree.Variables, v': CoordinationBetree.Variables, lbl: CoordinationBetree.TransitionLabel)
+  //   requires Inv(v)
+  //   requires CoordinationBetree.Next(v, v', lbl)
+  //   requires lbl.LoadEphemeralFromPersistentLabel? ==> AllocationBetreeRefinement.ValidStampedBetree(v.persistent)
+  //   requires lbl.InternalLabel? ==> AllocationBetreeRefinement.FreshLabel(v.ephemeral.v, AllocLbl(v, v', lbl))
+  //   ensures Inv(v')
+  // {
+  //   match lbl {
+  //     case LoadEphemeralFromPersistentLabel(_) => {
+  //       AllocationBetreeRefinement.InitRefines(v'.ephemeral.v, v.persistent);
+  //     }
+  //     case PutRecordsLabel(records) => {}
+  //     case QueryLabel(endLsn, key, value) => {}
+  //     case FreezeAsLabel(unobserved) => {}
+  //     case InternalLabel(allocs, deallocs) => {}
+  //   // | CommitStartLabel(newBoundaryLsn: LSN)
+  //   // | CommitCompleteLabel()
+  //   // | CrashLabel()
+  //     case _ => assume false;
+  //   } 
+  // }
+
+  predicate AllocBetreeRefineCondition(v: AllocationBetreeMod.Variables, lbl: AllocationBetreeMod.TransitionLabel)
+  {
+    && AllocationBetreeRefinement.FreshLabel(v, lbl)
+  }
+
+  lemma NextRefines(v: CoordinationBetree.Variables, v': CoordinationBetree.Variables, lbl: CoordinationBetree.TransitionLabel)
+    requires Inv(v)
+    requires CoordinationBetree.Next(v, v', lbl)
+    requires lbl.InternalLabel? ==> AllocBetreeRefineCondition(v.ephemeral.v, AllocLbl(v, v', lbl))
+    ensures Inv(v')
+    ensures CrashTolerantMap.Next(I(v), I(v'), ILbl(lbl))
+  {
+    assume false;
+    // match lbl {
+    //   case LoadEphemeralFromPersistentLabel() => {}
+    //   case ReadForRecoveryLabel(records) => { AllocNextRefinesAbstract(v.ephemeral.v, v'.ephemeral.v, AllocLbl(v, v', lbl)); }
+    //   case QueryEndLsnLabel(_) => {}
+    //   case PutLabel(_) => { AllocNextRefinesAbstract(v.ephemeral.v, v'.ephemeral.v, AllocLbl(v, v', lbl)); }
+    //   case InternalLabel(allocs, deallocs) => { AllocNextRefinesAbstract(v.ephemeral.v, v'.ephemeral.v, AllocLbl(v, v', lbl)); }
+    //   case QueryLsnPersistenceLabel(_) => {}
+    //   case FreezeAsLabel(_) => {}
+    //   case CommitStartLabel(_, _) => { AllocNextRefinesAbstract(v.ephemeral.v, v'.ephemeral.v, AllocLbl(v, v', lbl)); }
+    //   case CommitCompleteLabel(_, _)=> { AllocNextRefinesAbstract(v.ephemeral.v, v'.ephemeral.v, AllocLbl(v, v', lbl)); }
+    //   case CrashLabel() => {}
+    // }
+  }
+}
